Revising the concept of predicated messages

src/Prototype/Language.v
@@ -10,17 +10,17 @@ Section Language.
   Definition IdxT := nat.
 
   (* A message is always either a request or a response. *)
-  Inductive MsgType := Rq | Rs.
-  
+  Inductive RqRs := Rq | Rs.
+
   (** Utilities *)
   Definition idx_add {A} (k: IdxT) (v: A) m := add eq_nat_dec k v m.
-  Definition idx_msgType_dec: forall (k1 k2: IdxT * MsgType), {k1 = k2} + {k1 <> k2}.
+  Definition idx_msgType_dec: forall (k1 k2: IdxT * RqRs), {k1 = k2} + {k1 <> k2}.
   Proof.
     decide equality.
     - decide equality.
     - apply eq_nat_dec.
   Defined.
-  Definition idx_msgType_add {A} (k: IdxT * MsgType) (v: A) m :=
+  Definition idx_msgType_add {A} (k: IdxT * RqRs) (v: A) m :=
     add idx_msgType_dec k v m.
   Definition idx_idx_dec: forall (k1 k2: IdxT * IdxT), {k1 = k2} + {k1 <> k2}.
   Proof.
@@ -29,153 +29,90 @@ Section Language.
   Definition idx_idx_add {A} (k: IdxT * IdxT) (v: A) m :=
     add idx_idx_dec k v m.
 
-  (* Used in a whole system *)
-  Variable MsgT: MsgType -> Type.
+  Variable MsgT: Type.
   Variable StateT: Type.
 
-  (* [TrsLock] defines a lock for a transaction.
-   * Frequently we need to restrict behavior of an object between a certain 
-   * request and a following response. [TrsLock] can be used at this moment.
-   * The reason for the separation of [TrsLock]s and an object state is for
-   * easy verification, especially for the correctness of interleaving
-   * (linearizability).
-   *)
-  Inductive TLock ValueT :=
-  | TUnlocked : TLock ValueT
-  | TLocked : ValueT -> TLock ValueT.
-
-  (* Big TODO: need to generalize below fixed record type. 
-   * When the language is designed and following semantics are defined as a state
-   * transition relation, then each lock may be able to have its own type.
-   *)
-  Record LockElts :=
-    { le_idx : IdxT;
-      le_val : nat;
-      le_flag : bool
-    }.
-  Definition TrsLock := TLock LockElts. (* TODO: need to generalize *)
-  Definition TrsLocks := Map (IdxT (* rq *) * IdxT (* rs *)) TrsLock.
-
-  Section Message.
-    Record Msg := { msg_rq : IdxT; (* an object that requests this message *)
+  Record MsgId := { msg_rq : IdxT; (* an object that requests this message *)
                     msg_rs : IdxT; (* an object that responses this message *)
-                    msg_type : MsgType;
-                    msg_content : MsgT msg_type }.
+                    msg_rqrs : RqRs;
+                    msg_type : MsgT
+                  }.
 
-    Definition msgFrom (msg: Msg) :=
-      match msg_type msg with
-      | Rq => msg_rq msg
-      | Rs => msg_rs msg
-      end.
+  Definition msgFrom (msg: MsgId) :=
+    match msg_rqrs msg with
+    | Rq => msg_rq msg
+    | Rs => msg_rs msg
+    end.
 
-    Definition msgTo (msg: Msg) :=
-      match msg_type msg with
-      | Rq => msg_rs msg
-      | Rs => msg_rq msg
-      end.
+  Definition msgTo (msg: MsgId) :=
+    match msg_rqrs msg with
+    | Rq => msg_rs msg
+    | Rs => msg_rq msg
+    end.
 
-    Definition buildMsg rq rs {ty} (co: MsgT ty) :=
-      {| msg_rq := rq; msg_rs := rs;
-         msg_type := ty; msg_content := co |}.
+  Definition buildMsgId rq rs rr ty :=
+    {| msg_rq := rq; msg_rs := rs; msg_rqrs := rr; msg_type := ty |}.
 
-    Inductive PredMsg :=
-    | PmRq: forall (msg: Msg)
-                   (* Right after the request is sent, this lock is activated. *)
-                   (olock: option TrsLock)
-                   (* In order to handle the request, [precond] should be satisfied. *)
-                   (precond: StateT -> TrsLocks -> Prop), PredMsg
-    | PmRs: forall (msg: Msg), PredMsg.
+  (* [PmIn] represents messages both from external world and the internal system.
+   * [PmExtOut] is only for external requests/responses.
+   *)
+  Inductive PMsg :=
+  | PmIn: forall (msg: MsgId)
+                 (precond: StateT -> Prop)
+                 (outs: StateT -> list PMsg)
+                 (postcond: StateT -> Prop), PMsg
+  | PmExtOut: forall (msg: MsgId), PMsg.
 
-    Definition msgOf (pmsg: PredMsg) :=
-      match pmsg with
-      | PmRq msg _ _ => msg
-      | PmRs msg => msg
-      end.
+  Definition midOf (pmsg: PMsg) :=
+    match pmsg with
+    | PmIn msg _ _ _ => msg
+    | PmExtOut msg => msg
+    end.
 
-    Definition precondOf (pmsg: PredMsg) :=
-      match pmsg with
-      | PmRq _ _ precond => precond
-      | PmRs _ => fun _ _ => True
-      end.
+  Definition precondOf (pmsg: PMsg) :=
+    match pmsg with
+    | PmIn _ precond _ _ => precond
+    | PmExtOut _ => fun _ => True
+    end.
 
-  End Message.
+  Definition outsOf (pmsg: PMsg) :=
+    match pmsg with
+    | PmIn _ _ outs _ => outs
+    | PmExtOut _ => fun _ => nil
+    end.
 
-  Section Object.
-    
-    (* About rules:
-     * 1) For output messages, it's more accurate to have a type of [set Msg],
-     *    but it's fine if no two messages have the same receiver [msg_to].
-     *    This condition should be the part of well-formedness later.
-     * 2) A rule doesn't need to give the post [TrsLocks] state, locks are 
-     *    automatically held/released by transactions.
-     *)
-    Definition Rule :=
-      Msg -> TrsLocks -> StateT ->
-      option (list PredMsg (* messages out *) * StateT (* next state *)).
+  Definition postcondOf (pmsg: PMsg) :=
+    match pmsg with
+    | PmIn _ _ _ postcond => postcond
+    | PmExtOut _ => fun _ => True
+    end.
 
-    Record Object :=
-      { obj_idx: nat;
-        obj_state_init: StateT;
-        obj_rules: list Rule;
-      }.
+  Record Object :=
+    { obj_idx: nat;
+      obj_state_init: StateT;
+      obj_exts_allowed: MsgId -> Prop (* external messages that this object can handle *)
+    }.
 
-    Definition Objects := list Object.
-
-  End Object.
+  Definition Objects := list Object.
 
   Section Semantics.
 
-    Record ObjectState :=
-      { os_st: StateT;
-        (* list of (request, lock) *)
-        os_trs_locks: list (Msg * TrsLock)
-      }.
-    Fixpoint locksOf (ls: list (Msg * TrsLock)) :=
-      match ls with
-      | nil => @empty _ _
-      | (msg, l) :: ls' => idx_idx_add (msg_rq msg, msg_rs msg) l (locksOf ls')
-      end.
-
-    Definition isPair (m1 m2: Msg) :=
+    (* Has a record structure in case of more elements are required. *)
+    Record ObjectState := { os_st: StateT }.
+    
+    Definition isPair (m1 m2: MsgId) :=
       (if eq_nat_dec (msg_rq m1) (msg_rq m2) then true else false)
         && (if eq_nat_dec (msg_rs m1) (msg_rs m2) then true else false)
-        && (match msg_type m1, msg_type m2 with
+        && (match msg_rqrs m1, msg_rqrs m2 with
             | Rq, Rs => true
             | Rs, Rq => true
             | _, _ => false
             end).
 
-    Fixpoint addLocks (msgs_out: list PredMsg) (locks: list (Msg * TrsLock)) :=
-      match msgs_out with
-      | nil => locks
-      | msg_out :: msgs_out' =>
-        match msg_out with
-        | PmRq msg (Some lock) precond => addLocks msgs_out' ((msg, lock) :: locks)
-        | _ => addLocks msgs_out' locks
-        end
-      end.
-
-    Fixpoint removeLock (rs: Msg) (locks: list (Msg * TrsLock)) :=
-      match locks with
-      | nil => nil
-      | (rq, lock) :: locks =>
-        if isPair rs rq
-        then locks
-        else (rq, lock) :: (removeLock rs locks)
-      end.
-
-    Definition manageLock (msg_in: PredMsg) (msgs_out: list PredMsg)
-               (locks: list (Msg * TrsLock)) (st: StateT) :=
-      let alocks := addLocks msgs_out locks in
-      match msg_in with
-      | PmRs msg => removeLock msg alocks
-      | _ => alocks
-      end.
-
     Definition ObjectStates := Map IdxT ObjectState.
 
     Definition MsgsFrom :=
-      Map (IdxT * MsgType) (* (from, msgType) *) (list PredMsg).
+      Map (IdxT * RqRs) (* (from, msgType) *) (list PMsg).
     Definition Messages := Map IdxT (* to *) MsgsFrom.
 
     (* Note that [StepObjExt] takes an arbitrary message [emsg_in] as an input
@@ -184,46 +121,43 @@ Section Language.
      *)
     Inductive step_obj (obj: Object):
       ObjectState -> MsgsFrom ->
-      PredMsg (* in *) -> bool (* is_internal *) -> list PredMsg (* outs *) ->
+      PMsg (* in *) -> bool (* is_internal *) -> list PMsg (* outs *) ->
       ObjectState -> MsgsFrom -> Prop :=
-    | StepObjInt: forall os msgs_from fidx fpmsgT fpmsg fpmsgs msgs_out pos rule,
+    | StepObjInt: forall os msgs_from fidx fpmsgT fpmsg fpmsgs pos,
         find (fidx, fpmsgT) msgs_from = Some (fpmsg :: fpmsgs) ->
-        msgTo (msgOf fpmsg) = obj_idx obj ->
-        precondOf fpmsg (os_st os) (locksOf (os_trs_locks os)) ->
-        In rule (obj_rules obj) ->
-        rule (msgOf fpmsg) (locksOf (os_trs_locks os)) (os_st os) = Some (msgs_out, pos) ->
+        msgTo (midOf fpmsg) = obj_idx obj ->
+        precondOf fpmsg (os_st os) ->
+        postcondOf fpmsg pos ->
         step_obj obj os msgs_from
-                 fpmsg true msgs_out
-                 {| os_st := pos;
-                    os_trs_locks := manageLock fpmsg msgs_out (os_trs_locks os) (os_st os) |}
+                 fpmsg true (outsOf fpmsg (os_st os))
+                 {| os_st := pos |}
                  (idx_msgType_add (fidx, fpmsgT) fpmsgs msgs_from)
-    | StepObjExt: forall os msgs_from epmsg msgs_out pos rule,
-        msgTo (msgOf epmsg) = obj_idx obj ->
-        precondOf epmsg (os_st os) (locksOf (os_trs_locks os)) ->
-        In rule (obj_rules obj) ->
-        rule (msgOf epmsg) (locksOf (os_trs_locks os)) (os_st os) = Some (msgs_out, pos) ->
+    | StepObjExt: forall os msgs_from epmsg pos,
+        obj_exts_allowed obj (midOf epmsg) ->
+        msgTo (midOf epmsg) = obj_idx obj ->
+        precondOf epmsg (os_st os) ->
+        postcondOf epmsg pos ->
         step_obj obj os msgs_from
-                 epmsg false msgs_out
-                 {| os_st := pos;
-                    os_trs_locks := manageLock epmsg msgs_out (os_trs_locks os) (os_st os) |}
+                 epmsg false (outsOf epmsg (os_st os))
+                 {| os_st := pos |}
                  msgs_from.
 
-    Definition distributeMsg (from: IdxT) (pmsg: PredMsg)
+    Definition distributeMsg (from: IdxT) (pmsg: PMsg)
                (msgs: Messages): Messages :=
-      let msg := msgOf pmsg in
+      let msg := midOf pmsg in
       let to := msgTo msg in
       match find to msgs with
       | Some toMsgs =>
-        let added := match toMsgs (from, msg_type msg) with
+        let added := match toMsgs (from, msg_rqrs msg) with
                      | Some fromMsgs => fromMsgs ++ (pmsg :: nil)
                      | None => pmsg :: nil
                      end in
-        idx_add to (idx_msgType_add (from, msg_type msg) added toMsgs) msgs
+        idx_add to (idx_msgType_add (from, msg_rqrs msg) added toMsgs) msgs
       | None =>
-        idx_add to (idx_msgType_add (from, msg_type msg) (pmsg :: nil) (@empty _ _)) msgs
+        idx_add to (idx_msgType_add (from, msg_rqrs msg) (pmsg :: nil) (@empty _ _)) msgs
       end.
 
-    Fixpoint distributeMsgs (from: IdxT) (pmsgs: list PredMsg)
+    Fixpoint distributeMsgs (from: IdxT) (pmsgs: list PMsg)
              (msgs: Messages): Messages :=
       match pmsgs with
       | nil => msgs
@@ -232,8 +166,17 @@ Section Language.
 
     Definition getIndices (obs: Objects) := map (fun o => obj_idx o) obs.
 
+    Definition isExternal (indices: list nat) (pmsg: PMsg) :=
+      if in_dec eq_nat_dec (msgFrom (midOf pmsg)) indices
+      then false else true.
+
+    Definition getExt (indices: list nat) (pmsg: PMsg) :=
+      if isExternal indices pmsg then Some pmsg else None.
+    Definition getExts (indices: list nat) (msgs: list PMsg) :=
+      filter (fun pm => isExternal indices pm) msgs.
+
     Inductive step (obs: Objects) : ObjectStates -> Messages ->
-                                    PredMsg (* in *) -> list PredMsg (* outs *) ->
+                                    option PMsg (* ext_in *) -> list PMsg (* ext_outs *) ->
                                     ObjectStates -> Messages -> Prop :=
     | Step: forall oss idx (obj: Object) (os: ObjectState)
                    oims msgs_from msg_in is_internal msgs_out pos pmsgs_from,
@@ -242,16 +185,23 @@ Section Language.
         find idx oss = Some os ->
         find idx oims = Some msgs_from -> 
         step_obj obj os msgs_from msg_in is_internal msgs_out pos pmsgs_from ->
-        is_internal = (if in_dec eq_nat_dec (msgFrom (msgOf msg_in)) (getIndices obs)
-                       then true else false) ->
+        is_internal = negb (isExternal (getIndices obs) msg_in) ->
         step obs oss oims
-             msg_in msgs_out
+             (getExt (getIndices obs) msg_in)
+             (getExts (getIndices obs) msgs_out)
              (idx_add idx pos oss)
              (distributeMsgs idx msgs_out (idx_add idx pmsgs_from oims)).
 
+    Definition ocons {A} (oa: option A) (l: list A) :=
+      match oa with
+      | Some a => a :: l
+      | None => l
+      end.
+    Infix "::>" := ocons (at level 0).
+
     (* Head is the oldest message. *)
     Inductive steps (obs: Objects) : ObjectStates -> Messages ->
-                                     list PredMsg (* history *) ->
+                                     list PMsg (* history *) ->
                                      ObjectStates -> Messages -> Prop :=
     | StepsNil: forall oss oims, steps obs oss oims nil oss oims
     | StepsCons:
@@ -259,26 +209,25 @@ Section Language.
           steps obs oss1 oims1 emsgs oss2 oims2 ->
           forall oss3 msg_in msgs_out oims3,
             step obs oss2 oims2 msg_in msgs_out oss3 oims3 ->
-            steps obs oss1 oims1 (emsgs ++ msg_in :: msgs_out) oss3 oims3.
+            steps obs oss1 oims1 (emsgs ++ msg_in ::> msgs_out) oss3 oims3.
 
     Fixpoint getObjectStatesInit (obs: Objects) : ObjectStates :=
       match obs with
       | nil => @empty _ _
       | obj :: obs' =>
         idx_add (obj_idx obj)
-                {| os_st := obj_state_init obj; os_trs_locks := nil |}
+                {| os_st := obj_state_init obj |}
                 (getObjectStatesInit obs')
       end.
 
-    Inductive HistoryOf : Objects -> list PredMsg -> Prop :=
+    Inductive HistoryOf : Objects -> list PMsg -> Prop :=
     | History:
         forall obs oss oims phst,
           steps obs (getObjectStatesInit obs) (@empty _ _) phst oss oims ->
           HistoryOf obs phst.
 
     (* A history consisting only of requests and matching responses. *)
-    (** TODO: better definition? *)
-    Inductive Complete: list Msg -> Prop :=
+    Inductive Complete: list MsgId -> Prop :=
     | CplNil: Complete nil
     | CplAdd:
         forall hst1 hst2 hst3,
@@ -289,12 +238,21 @@ Section Language.
               chst = hst1 ++ rq :: hst2 ++ rs :: hst3 ->
               Complete chst.
 
+    Inductive SubList {A}: list A -> list A -> Prop :=
+    | SlNil: SubList nil nil
+    | SlAdd: forall l1 l2, SubList l1 l2 -> forall a, SubList (a :: l1) (a :: l2)
+    | SlSkip: forall l1 l2, SubList l1 l2 -> forall a, SubList l1 (a :: l2).
+
+    Definition complete (hst chst: list MsgId): Prop :=
+      Complete chst /\ SubList chst hst /\
+      (* maximal *) forall hst', Complete hst' -> SubList hst' hst -> ~ SubList chst hst'.
+
     (* An informal definition of "sequential":
      * 1) The first message should be a request
      * 2) A matching response for each request should be right after the request.
      * 3) There might not be a matching response for the last request.
      *)
-    Inductive CSequential: list Msg -> Prop :=
+    Inductive CSequential: list MsgId -> Prop :=
     | CseqNil: CSequential nil
     | CseqAdd:
         forall hst,
@@ -305,12 +263,12 @@ Section Language.
               chst = hst ++ rq :: rs :: nil ->
               CSequential chst.
 
-    Inductive Sequential: list Msg -> Prop :=
+    Inductive Sequential: list MsgId -> Prop :=
     | SeqCompl: forall hst, CSequential hst -> Sequential hst
     | SeqIncom:
         forall hst,
           CSequential hst ->
-          forall rq, msg_type rq = Rq ->
+          forall rq, msg_rqrs rq = Rq ->
                      Sequential (hst ++ rq :: nil).
 
     (* In message passing system, "object subhistory" and "process subhistory"
@@ -320,39 +278,42 @@ Section Language.
      * For requests, j's subhistory contains them.
      * For responses, i's subhistory contains them.
      *)
-    Definition isObjectsMsg (obs: list IdxT) (e: Msg) :=
-      (if in_dec idx_msgType_dec (msg_rq e, msg_type e)
+    Definition isObjectsMsg (obs: list IdxT) (e: MsgId) :=
+      (if in_dec idx_msgType_dec (msg_rq e, msg_rqrs e)
                  (map (fun i => (i, Rq)) obs) then true else false)
-        || (if in_dec idx_msgType_dec (msg_rs e, msg_type e)
+        || (if in_dec idx_msgType_dec (msg_rs e, msg_rqrs e)
                       (map (fun i => (i, Rs)) obs) then true else false).
-    Definition objSubHistory (i: IdxT) (hst: list Msg) :=
+    Definition objSubHistory (i: IdxT) (hst: list MsgId) :=
       filter (isObjectsMsg (i :: nil)) hst.
 
-    Definition intHistory (internals: list IdxT) (hst: list Msg) :=
+    Definition intHistory (internals: list IdxT) (hst: list MsgId) :=
       filter (isObjectsMsg internals) hst.
-    Definition extHistory (internals: list IdxT) (hst: list Msg) :=
+    Definition extHistory (internals: list IdxT) (hst: list MsgId) :=
       filter (fun e => negb (isObjectsMsg internals e)) hst.
 
     (* Two histories are equivalent iff any object subhistories are equal. *)
-    Definition Equivalent (hst1 hst2: list Msg) :=
+    Definition Equivalent (hst1 hst2: list MsgId) :=
       forall i, objSubHistory i hst1 = objSubHistory i hst2.
 
     (* TODO: this is actually not a fully correct definition:
-     * 1) Instead of [Equivalent hst lhst], we need [Equivalent (complete hst) lhst]
+     * 1) [complete] definition is a bit different to the one in original
+     * definition, but I think it's enough. Need to confirm whether it's indeed
+     * the right definition.
      * 2) Linearizability requires one more condition: any _strict_ transaction
-     *    orders are preserved by [lhst].
+     * orders are preserved by [lhst].
      *)
-    Definition Linearizable' (hst lhst: list Msg) :=
-      Sequential lhst /\ Equivalent hst lhst.
+    Definition Linearizable' (hst lhst: list MsgId) :=
+      Sequential lhst /\
+      exists chst, complete hst chst /\ Equivalent chst lhst.
 
-    Definition Linearizable (hst: list Msg) :=
+    Definition Linearizable (hst: list MsgId) :=
       exists lhst, Linearizable' hst lhst.
 
-    Definition AbsLinear (obs: Objects) (absF: list Msg -> list Msg) :=
+    Definition AbsLinear (obs: Objects) (absF: list MsgId -> list MsgId) :=
       forall hst,
         HistoryOf obs hst ->
         exists shst, HistoryOf obs shst /\
-                     Linearizable' (absF (map msgOf hst)) (absF (map msgOf shst)).
+                     Linearizable' (absF (map midOf hst)) (absF (map midOf shst)).
 
     Definition IntLinear (obs: Objects) :=
       AbsLinear obs (intHistory (getIndices obs)).
@@ -364,14 +325,16 @@ Section Language.
       forall hst,
         HistoryOf obs hst ->
         exists shst, HistoryOf obs shst /\
-                     Linearizable' (map msgOf hst) (map msgOf shst).
+                     Linearizable' (map midOf hst) (map midOf shst).
 
   End Semantics.
 
   Section Facts.
 
     Lemma equivalent_refl: forall hst, Equivalent hst hst.
-    Proof. intros; unfold Equivalent; reflexivity. Qed.
+    Proof.
+      intros; unfold Equivalent; reflexivity.
+    Qed.
     Hint Immediate equivalent_refl.
 
   End Facts.
